\subsection{Determination of $R_{eq}$}
\label{section:R}
Just as suggested, we made $V_s = 0$ and replaced the capacitor with a voltage source $V_x= V(6)-V(8)$, where V(6) and V(8) are the voltages in nodes 6 and 8 as obtained in section ~\ref{}. Then, we made once again the nodal analysis, with the purpose of obtaining values for $I_x$ and $V-x$. Now, we only need 6 equations, because the GND node and node 1 become the same node.\\
For node 2, we get:
\begin{equation}
\frac{V_2}{R_1} + \frac{V_2 - V_3}{R_2} + \frac{V_2 - V_5}{R_3} = 0 \Leftrightarrow V_2\left( \frac{1}{R_1} + \frac{1}{R_2} + \frac{1}{R_3} \right) - \frac{V_3}{R_2} - \frac{V_5}{R_3}=0
\end{equation}

For node 3, remembering the equation (A DO IB):
\begin{equation}
\frac{V_3 - V_2}{R_2\times K_b }+ V_5 - V_2 = 0 \Leftrightarrow V_2 \left(-\frac{1}{R_2\times K_b} - 1\right) + \frac{V_3}{R_2\times K_b} + V_5 = 0
\end{equation}

For node 5:
\begin{equation}
\frac{V_5}{R_4}+ \frac{V_5-V_2}{R_3} + \frac{V_5-V_6}{R_5} + i_d= 0 
\end{equation}

Where $i_d$ is the current passing trough the dependent voltage source $V_d$ ($i_d = -(I_d + I_x)$).

For node 6 (remebering the equation A DO IB)we get:
\begin{equation}
I_b + \frac{V_6-V_5}{R_5} + I_x = 0 \Leftrightarrow I_x = \frac{V_2-V_3}{R_2} + \frac{V_5-V_6}{R_5}
\end{equation}

And also:
\begin{equation}
V_6-V_8 = V_x
\end{equation}

For node 7:
\begin{equation}
V7x==R6*((V8x - V7x)/R7);
-I_d + \frac{V_7-V_8}{R_7} = 0 \Leftrightarrow \frac{V_7}{R_6} - \frac{V_7-V_8}{R_7} = 0\Leftrightarrow V_7\left(\frac{1}{R_6} + \frac{1}{R_7}\right) - \frac{V_8}{R_7} = 0
\end{equation}

Combinig equations (a do nodo 5), (primeira do nodo 6) and noticing that $I_d = \frac{V_7-V_8}{R_7}$:
\begin{equation}
V_2 \left( -\frac{1}{R_2} - \frac{1}{R_3}\right) + \frac{V_3}{R_2} +  V_5 \left( \frac{1}{R_3} + \frac{1}{R_4}\right) - \frac{V_7}{R_7} + \frac{V_8}{R_7} = 0
\end{equation}

Knowing that $I_d = \frac{V_d}{K_d}$ and $I_d = \frac{V_7-V_8}{R_7}$, we get the final equation:
\begin{equation}
V_8\left( \frac{1}{R_7} - \frac{1}{K_d}\right) - \frac{V_7}{R_7} + \frac{V_5}{K_d}
\end{equation}


The next step is to solve the following system of equations:
\begin{equation}
\left(\begin{array}{cccccc} \frac{1}{R_1}+\frac{1}{R_2} +\frac{1}{R_3} & -\frac{1}{R_2} & -\frac{1}{R_3} & 0 & 0 & 0\\ -\frac{1}{R_2\times K_b}-1 & \frac{1}{R_2\times K_b} & 1 & 0 & 0 & 0 \\ -\frac{1}{R_2}-\frac{1}{R_3} & \frac{1}{R_2} & \frac{1}{R_3}+\frac{1}{R_4} & 0& -\frac{1}{R_7} &\frac{1}{R_7} \\ 0&0&0&1&0&-1\\0&0&0&0&\frac{1}{R_6}+\frac{1}{R_7}&-\frac{1}{R_7} \\ 0&0&\frac{1}{K_d}&0&-\frac{1}{R_7}&\frac{1}{R_7}-\frac{1}{K_d}\end{array}\right)
\left(\begin{array}{c} V_2 \\ V_3 \\ V_5 \\ V_6 \\ V_7 \\ V_8 \end{array}\right) 
= \left(\begin{array}{c} 0 \\ 0 \\ 0 \\ V_x \\ 0 \\ 0 \end{array}\right)
\end{equation}

Finally, we can calculate $I_x$ using equation (VER), the equivalent resistance $R_{eq}$ and the time constant, $\tau$: 
\begin{equation}
R_{eq}=-\frac{V_x}{I_x}
\end{equation}
\begin{equation}
\tau=\frac{R_{eq}\times C}{1000}
\end{equation}